<?xml version="1.0" encoding="utf-8"?>
<rdf:RDF
   xmlns:dc="http://purl.org/dc/elements/1.1/"
   xmlns:dct="http://purl.org/dc/terms/"
   xmlns:ldproc="https://doi.org/10.6069/uwlib.55.b.2#"
   xmlns:rdf="http://www.w3.org/1999/02/22-rdf-syntax-ns#"
   xmlns:rdfs="http://www.w3.org/2000/01/rdf-schema#"
   xmlns:schema="https://schema.org/"
   xmlns:void="http://rdfs.org/ns/void#"
>
  <rdf:Description rdf:about="https://doi.org/10.6069/uwlib.55.d.1">
    <rdf:type rdf:resource="http://rdfs.org/ns/void#Dataset"/>
    <dct:creator rdf:resource="http://viaf.org/viaf/139541794"/>
    <dc:creator xml:lang="en">University of Washington Libraries</dc:creator>
    <dct:publisher rdf:resource="http://viaf.org/viaf/139541794"/>
    <dc:publisher xml:lang="en">University of Washington Libraries</dc:publisher>
    <dct:title xml:lang="en">University of Washington Libraries rdfs:Class Definitions</dct:title>
    <dct:description xml:lang="en">RDF dataset describing classes used in University of Washington Libraries RDF data.</dct:description>
    <void:feature rdf:resource="http://www.w3.org/ns/formats/RDFa"/>
    <void:feature rdf:resource="http://www.w3.org/ns/formats/N-Triples"/>
    <void:feature rdf:resource="http://www.w3.org/ns/formats/RDF_XML"/>
    <void:feature rdf:resource="http://www.w3.org/ns/formats/Turtle"/>
    <ldproc:containsEntity rdf:resource="http://www.w3.org/2000/01/rdf-schema#Class"/>
    <void:classPartition rdf:nodeID="N656363c278f24f6b90e311aadce2402c"/>
    <schema:version>1-2-1</schema:version>
    <dct:hasFormat rdf:resource="https://uwlib-cams.github.io/uwlswd_vocabs/university_of_washington_libraries_rdfsclass_definitions/university_of_washington_libraries_rdfsclass_definitions.ttl"/>
    <dct:hasFormat rdf:resource="https://uwlib-cams.github.io/uwlswd_vocabs/university_of_washington_libraries_rdfsclass_definitions/university_of_washington_libraries_rdfsclass_definitions.nt"/>
    <dct:hasFormat rdf:resource="https://uwlib-cams.github.io/uwlswd_vocabs/university_of_washington_libraries_rdfsclass_definitions/university_of_washington_libraries_rdfsclass_definitions.jsonld"/>
    <dct:hasFormat rdf:resource="https://uwlib-cams.github.io/uwlswd_vocabs/university_of_washington_libraries_rdfsclass_definitions/university_of_washington_libraries_rdfsclass_definitions.html"/>
  </rdf:Description>
  <rdf:Description rdf:about="https://doi.org/10.6069/uwlib.55.d.1#NegativeNumber">
    <rdf:type rdf:resource="http://www.w3.org/2000/01/rdf-schema#Class"/>
    <rdfs:isDefinedBy rdf:resource="https://doi.org/10.6069/uwlib.55.d.1"/>
    <rdfs:subClassOf rdf:resource="http://id.loc.gov/ontologies/bibframe/Identifier"/>
    <rdfs:label xml:lang="en">Negative Number</rdfs:label>
    <rdfs:comment xml:lang="en">Reproduction number assigned to an image for purposes of
      duplication. It is a unique number in University of Washington Libraries Special
      Collections.</rdfs:comment>
  </rdf:Description>
  <rdf:Description rdf:about="https://doi.org/10.6069/uwlib.55.d.1#PhotographersReferenceNumber">
    <rdf:type rdf:resource="http://www.w3.org/2000/01/rdf-schema#Class"/>
    <rdfs:isDefinedBy rdf:resource="https://doi.org/10.6069/uwlib.55.d.1"/>
    <rdfs:subClassOf rdf:resource="http://id.loc.gov/ontologies/bibframe/Identifier"/>
    <rdfs:label xml:lang="en">Photographers Reference Number</rdfs:label>
    <rdfs:comment xml:lang="en">University of Washington Libraries' reference number for a
      photographer.</rdfs:comment>
  </rdf:Description>
  <rdf:Description rdf:about="https://doi.org/10.6069/uwlib.55.d.1#OrderNumber">
    <rdf:type rdf:resource="http://www.w3.org/2000/01/rdf-schema#Class"/>
    <rdfs:isDefinedBy rdf:resource="https://doi.org/10.6069/uwlib.55.d.1"/>
    <rdfs:subClassOf rdf:resource="http://id.loc.gov/ontologies/bibframe/Identifier"/>
    <rdfs:label xml:lang="en">Order Number</rdfs:label>
    <rdfs:comment xml:lang="en">Number used to order a copy of a digital resource from the
      University of Washington Libraries.</rdfs:comment>
  </rdf:Description>
  <rdf:Description rdf:nodeID="N656363c278f24f6b90e311aadce2402c">
    <void:class rdf:resource="http://www.w3.org/2000/01/rdf-schema#Class"/>
  </rdf:Description>
</rdf:RDF>
